Monotonicity of strategy aggregation

games/MultiChannel.v
@@ -1,5 +1,6 @@
 Require Import LogicalRelations.
 Require Import KLR.
+Require Import List.
 Require Import Classical.
 Require Import ClassicalChoice.
 Require Import DecidableClass.
@@ -45,7 +46,7 @@ Module Pow.
     Context {GA GB I} {S K : I -> Type} (α : forall i, ats GA GB (S i) (K i)).
 
     Inductive state :=
-      st (i : I) (s : S i) (k : forall j, i <> j -> K j).
+      st (i : I) (s : S i) (k : forall j, K j).
 
     Definition cont :=
       forall i : I, K i.
@@ -58,14 +59,14 @@ Module Pow.
     Inductive suspend : state -> pmove (GA ^ I) (GB ^ I) * cont -> Prop :=
       suspend_intro i s k m ki k' :
         ATS.suspend (α i) s (m, ki) ->
-        (forall j Hj, k' j = k j Hj) ->
+        (forall j, i <> j -> k' j = k j) ->
         k' i = ki ->
         suspend (st i s k) (mkp i m, k').
 
     Inductive resume : cont -> omove (GA ^ I) (GB ^ I) -> state -> Prop :=
       resume_intro i k m s :
         ATS.resume (α i) (k i) m s ->
-        resume k (mko i m) (st i s (fun j _ => k j)).
+        resume k (mko i m) (st i s k).
 
     Inductive refuse : cont -> question (GB ^ I) -> Prop :=
       refuse_intro i k m :
@@ -77,53 +78,242 @@ Module Pow.
 
   End ATS.
 
-  Arguments state : clear implicits.
-  Arguments cont : clear implicits.
+  Arguments state {I} S K.
+  Arguments cont {I} K.
 
   (** ** Monotonicity *)
 
   (** We can build KLRs for these two kinds of maps. *)
 
-  (*
   Section REL.
-    Context {G1 G2} (GR : grel G1 G2) (I : Type).
-    Context {A1 A2} (RA : klr GR A1 A2).
-    Context {B1 B2} (RB : klr GR B1 B2).
+    Context {GA1 GA2} (GRA : grel GA1 GA2).
+    Context {GB1 GB2} (GRB : grel GB1 GB2).
+    Context (I : Type) `{forall i j : I, Decidable (i = j)}.
+    Context {S1 S2} (RS : forall i:I, klr (gworld GRA GRB) (S1 i) (S2 i)).
+    Context {K1 K2} (RK : forall i:I, klr (gworld GRA GRB) (K1 i) (K2 i)).
 
-    Definition unfocused_r : klr (GR^I)%grel (unfocused I A1) (unfocused I A2) :=
-      fun '(Pow.mkw w i) f1 f2 => forall i, RA (w i) (f1 i) (f2 i).
+    Definition sum_map {A1 A2} (f : A1 -> A2) {B1 B2} (g : B1 -> B2) :=
+      fun x : A1 + B1 =>
+        match x with
+          | inl a1 => inl (f a1)
+          | inr b1 => inr (g b1)
+        end.
 
-    Inductive focused_r : klr (GR ^ I)%grel _ _ :=
-      focused_r_intro w i b1 b2 f1 f2 :
-        RB (w i) b1 b2 ->
-        (forall j Hj, RA (w j) (f1 j Hj) (f2 j Hj)) ->
-        focused_r (Pow.mkw w i) (foc i b1 f1) (foc i b2 f2).
+    Inductive wfw : option I -> gworld (GRA ^ I) (GRB ^ I) -> Prop :=
+      | wfw_nil :
+          wfw None nil
+      | wfw_oq i w ws :
+          wfw None ws ->
+          wfw (Some i) (inr (i, w) :: ws)
+      | wfw_pq i w ws :
+          wfw (Some i) ws ->
+          wfw None (inl (i, w) :: ws).
 
-    Global Instance init_r :
-      Monotonic init ([] RA @@ [Pow.getw] ++> unfocused_r).
-    Admitted.
+    Fixpoint wproj i (ws : gworld (GRA ^ I) (GRB ^ I)) : gworld GRA GRB :=
+      match ws with
+        | nil => nil
+        | inl (j, w) :: ws' =>
+          if decide (j = i) then inl w :: wproj i ws' else wproj i ws'
+        | inr (j, w) :: ws' =>
+          if decide (j = i) then inr w :: wproj i ws' else wproj i ws'
+      end.
 
-    Global Instance focus_r :
-      Monotonic focus
-        (forallr - @ i,
-         |= unfocused_r ++>
-            k1 set_le (RA@@[Pow.getw] * ((<> RB@@[Pow.getw]) ++> <> focused_r))).
-    Admitted.
+    Inductive state_rel ws : rel (state S1 K1) (state S2 K2) :=
+      state_rel_intro i s1 s2 k1 k2 :
+        wfw (Some i) ws ->
+        RS i (wproj i ws) s1 s2 ->
+        (forall j, i <> j -> RK j (wproj j ws) (k1 j) (k2 j)) ->
+        state_rel ws (st i s1 k1) (st i s2 k2).
 
-    Global Instance update_r :
-      Monotonic update
-        (|= RB @@ [Pow.getw] ++> focused_r ++>
-            k1 set_le (k eq * RB @@ [Pow.getw] * focused_r)).
-    Admitted.
+    Definition cont_rel : klr (gworld (GRA^I) (GRB^I)) (cont K1) (cont K2) :=
+      fun ws k1 k2 =>
+        wfw None ws /\
+        forall i, RK i (wproj i ws) (k1 i) (k2 i).
 
-    Global Instance unfocus_r :
-      Monotonic unfocus
-        (|= focused_r ++>
-            k1 set_le (k eq * RB@@[Pow.getw] *
-                       ((<> RA@@[Pow.getw]) ++> <> unfocused_r))).
-    Admitted.
+    Lemma wproj_acc_o i mo1 m2 ws ws' :
+      wfw None ws ->
+      gacc (GRA ^ I) (GRB ^ I) (om (mko i mo1), m2) ws ws' ->
+      exists mo2,
+        m2 = om (mko i mo2) /\
+        wfw (Some i) ws' /\
+        gacc GRA GRB (om mo1, om mo2) (wproj i ws) (wproj i ws') /\
+        forall j, i <> j -> wproj j ws' = wproj j ws.
+    Proof.
+      intros Hws Hws'.
+      inversion Hws'; clear Hws'; subst.
+      - (* OQ *)
+        inversion H4; clear H4; subst.
+        destruct w0 as [j w], m1, m0. simpl in H2. destruct H2 as [His Hm].
+        simpl in His. destruct His. destruct mo1; inversion H0; clear H0; subst.
+        exists (oq q0). simpl in *. intuition auto.
+        + constructor; auto.
+        + rewrite Decidable_complete by auto.
+          repeat constructor; auto.
+        + rewrite Decidable_sound_alt by auto.
+          reflexivity.
+      - (* OA *)
+        inversion H4; clear H4; subst.
+        destruct w0 as [j w], m1, m0. simpl in H2. destruct H2 as [His Hm].
+        simpl in His. destruct His. destruct mo1; inversion H0; clear H0; subst.
+        exists (oa a0). simpl in *. intuition auto.
+        + inversion Hws; clear Hws; subst. auto.
+        + rewrite Decidable_complete by auto.
+          repeat constructor; auto.
+        + rewrite Decidable_sound_alt by auto.
+          reflexivity.
+    Qed.        
   End REL.
-*)
+
+  Global Instance step_sim :
+    Monotonic
+      (@step)
+      (forallr GRA, forallr GRB, forallr - @ I,
+       rforall Idec : (forall i j : I, Decidable (i = j)),
+       forallr RS : fun S1 S2 => forall i, klr _ (S1 i) (S2 i),
+       forallr RK : fun K1 K2 => forall i, klr _ (K1 i) (K2 i),
+       (forallr - @ i, ATS.sim GRA GRB (RS i) (RK i)) ++>
+       |=  state_rel GRA GRB I RS RK ++> k1 set_le (state_rel GRA GRB I RS RK)).
+  Proof.
+    intros GA1 GA2 GRA GB1 GB2 GRB I Idec S1 S2 RS K1 K2 RK.
+    intros α β Hαβ ws x1 x2 Hx x1' Hx1'. destruct Hx1' as [i s1 s1' k1 Hs1'].
+    inversion Hx; clear Hx. apply inj_pair2 in H0. subst.
+    edestruct @ATS.sim_step as (s2' & Hs2' & Hs'); eauto.
+    eexists. split.
+    - econstructor; eauto.
+    - econstructor; eauto.
+  Qed.
+
+  Axiom proof_irrelevance : forall (P:Prop) (p1 p2:P), p1 = p2.
+
+  Lemma update_contmap {I K} {Idec : forall i j : I, Decidable (i = j)} :
+    forall i ki (k : forall j:I, K j),
+      exists k' : (forall i:I, K i),
+        k' i = ki /\ forall j, i <> j -> k' j = k j.
+  Proof.
+    intros.
+    assert (Hchoi: ChoiceFacts.DependentFunctionalChoice_on K).
+    {
+      apply ChoiceFacts.non_dep_dep_functional_choice.
+      intros. intro. apply choice.
+    }
+    red in Hchoi.
+    destruct
+      (Hchoi (fun j k'j =>
+                (forall Hj, k'j = eq_rect i K ki j Hj) /\
+                (i <> j -> k'j = k j))) as
+      (k' & Hk').
+    {
+      clear. intros j. destruct (classic (i = j)).
+      - destruct H. exists ki. split; try congruence.
+        intros Hi. rewrite <- eq_rect_eq. reflexivity.
+      - exists (k j). split; congruence.
+    }
+    exists k'. split.
+    - specialize (Hk' i) as [H _]. specialize (H eq_refl). simpl in H. auto.
+    - intros j Hj. specialize (Hk' j) as [_ H]. specialize (H Hj). auto.
+  Qed.
+
+  (* TODO: split out wproj_acc_p as appropriate *)
+  Global Instance suspend_sim :
+    Monotonic
+      (@suspend)
+      (forallr GRA, forallr GRB, forallr - @ I,
+       rforall Idec : (forall i j : I, Decidable (i = j)),
+       forallr RS : fun S1 S2 => forall i, klr _ (S1 i) (S2 i),
+       forallr RK : fun K1 K2 => forall i, klr _ (K1 i) (K2 i),
+       (forallr - @ i, ATS.sim GRA GRB (RS i) (RK i)) ++>
+       |=  state_rel GRA GRB I RS RK ++>
+           k1 set_le (<> * cont_rel GRA GRB I RK)).
+  Proof.
+    intros GA1 GA2 GRA GB1 GB2 GRB I Idec S1 S2 RS K1 K2 RK.
+    intros α β Hαβ ws x1 x2 Hx x1' Hx1'.
+    destruct Hx1' as [i s1 k1 m1 ki1 k1' Hki1 Hk1' Hki1'].
+    inversion Hx; clear Hx. apply inj_pair2 in H0. subst.
+    edestruct @ATS.sim_suspend as ([m2 k2i'] & Hmk2 & Hmk); eauto.
+    destruct Hmk as (wi' & Hm & Hk).
+    destruct (update_contmap i k2i' k2) as (k2' & Hk2'i & Hk2'j).
+    exists (Pow.mkp i m2, k2'). split.
+    - econstructor; eauto.
+    - inversion Hm; clear Hm; subst.
+      + inversion H6; clear H6; subst.
+        exists (inl (i, w0) :: ws). split.
+        * repeat constructor; auto.
+        * split. { constructor. auto. }
+          intros j. simpl. destruct decide eqn:Hdec.
+          -- apply Decidable_sound in Hdec. subst. auto.
+          -- apply Decidable_complete_alt in Hdec.
+             assert (Hij : i <> j) by congruence.
+             erewrite (Hk1' _ Hij), (Hk2'j _ Hij).
+             auto.
+      + inversion H6; clear H6; subst.
+        inversion H2; clear H2; subst.
+        simpl in H3. rewrite Decidable_complete in H3 by auto.
+        inversion H3; clear H3; subst.
+        * exists ws0. split.
+          -- repeat constructor; auto.
+          -- split; auto. intro j.
+             specialize (H5 j). simpl wproj in H5.
+             destruct decide eqn:Hj.
+             ++ apply Decidable_sound in Hj. subst. auto.
+             ++ apply Decidable_complete_alt in Hj.
+                rewrite (Hk1' j Hj), (Hk2'j j Hj). auto.
+  Qed.
+
+  Global Instance resume_sim :
+    Monotonic
+      (@resume)
+      (forallr GRA, forallr GRB, forallr - @ I,
+       rforall Idec : (forall i j : I, Decidable (i = j)),
+       forallr RS : fun S1 S2 => forall i, klr _ (S1 i) (S2 i),
+       forallr RK : fun K1 K2 => forall i, klr _ (K1 i) (K2 i),
+       (forallr - @ i, ATS.sim GRA GRB (RS i) (RK i)) ++>
+       |=  cont_rel GRA GRB I RK ++> [] -> k1 set_le (state_rel GRA GRB I RS RK)).
+  Proof.
+    intros GA1 GA2 GRA GB1 GB2 GRB I Idec S1 S2 RS K1 K2 RK.
+    intros α β Hαβ ws k1 k2 Hk m1 m2 ws' Hm s1 Hs1.
+    destruct Hs1 as [i k1 m1 s1 Hs1].
+    destruct Hk as [Hws Hk].
+    eapply wproj_acc_o in Hm as (mo2 & Hm2 & Hws' & Hm & Hws'j); eauto.
+    inversion Hm2; clear Hm2; subst.
+    edestruct @ATS.sim_resume as (s2 & Hs2 & Hs); eauto. { eapply Hm. }
+    exists (st i s2 k2). split.
+    - constructor; auto.
+    - constructor; auto.
+      intros. rewrite Hws'j by auto. auto.
+  Qed.
+
+  Global Instance refuse_sim :
+    Monotonic
+      (@refuse)
+      (forallr GRA, forallr GRB, forallr - @ I,
+       rforall Idec : (forall i j : I, Decidable (i = j)),
+       forallr RS : fun S1 S2 => forall i, klr _ (S1 i) (S2 i),
+       forallr RK : fun K1 K2 => forall i, klr _ (K1 i) (K2 i),
+       (forallr - @ i, ATS.sim GRA GRB (RS i) (RK i)) ++>
+       |=  cont_rel GRA GRB I RK ++> [] -> k impl).
+  Proof.
+    intros GA1 GA2 GRA GB1 GB2 GRB I Idec S1 S2 RS K1 K2 RK.
+    intros α β Hαβ ws k1 k2 [Hws Hk] m1 m2 ws' Hm Hm1.
+    destruct Hm1 as [i k1 m1 Hm1].
+    apply (wproj_acc_o GRA GRB I i (oq m1)) in Hm; auto.
+    destruct Hm as (mo2 & Hm2 & Hws' & Hm & Hws'j).
+    destruct mo2; inversion Hm2; clear Hm2; subst.
+    constructor.
+    eapply @ATS.sim_refuse; eauto. apply Hm.
+  Qed.
+
+  Global Instance of_sim :
+    Monotonic
+      (@of)
+      (forallr GRA, forallr GRB, forallr - @ I,
+       rforall Idec : (forall i j : I, Decidable (i = j)),
+       forallr RS : fun S1 S2 => forall i, klr _ (S1 i) (S2 i),
+       forallr RK : fun K1 K2 => forall i, klr _ (K1 i) (K2 i),
+       (forallr - @ i, ATS.sim GRA GRB (RS i) (RK i)) ++>
+       ATS.sim (GRA^I) (GRB^I) (state_rel GRA GRB I RS RK) (cont_rel GRA GRB I RK)).
+  Proof.
+    split; simpl; rauto.
+  Qed.
 
 End Pow.
 
